ElemsCounts.ec
@@ -2,78 +2,75 @@
 
 (* Finite Maps Providing Counts for Certain Elements *)
 
-require import AllCore FSet NewFMap FMapAux.
+require import AllCore FSet SmtMap MapAux.
 
 (* counts for certain elements; counts are always >= 1 *)
 
-type 'a counts = ('a, int)fmap.
+type 'a counts = ('a, int) fmap.
 
 (* empty elements counts map *)
 
-op empty_counts : 'a counts = map0.
+op empty_counts : 'a counts = empty.
 
 (* when looking up a count, the result is 0 when not in map's domain *)
 
 op get_count (cnts : 'a counts) (elem : 'a) : int =
-  if mem (dom cnts) elem then oget cnts.[elem] else 0.
+  if elem \in cnts then oget cnts.[elem] else 0.
 
 (* when incrementing a count, if the element isn't already in the
    map's domain, we start at 1 *)
 
 op incr_count (cnts : 'a counts) (elem : 'a) : 'a counts =
-  if mem (dom cnts) elem
+  if elem \in cnts
   then cnts.[elem <- oget(cnts.[elem]) + 1]
   else cnts.[elem <- 1].
 
 (* lemmas about elements counts maps *)
 
 lemma ec_incr_mem_eq (cnts : 'a counts, elem : 'a) :
-  mem (dom cnts) elem =>
+  elem \in cnts =>
   incr_count cnts elem =
   cnts.[elem <- oget(cnts.[elem]) + 1].
 proof. rewrite /incr_count; by move => ->. qed.
 
 lemma ec_incr_not_mem_eq (cnts : 'a counts, elem : 'a) :
-  ! mem (dom cnts) elem =>
+  ! elem \in cnts =>
   incr_count cnts elem = cnts.[elem <- 1].
 proof. rewrite /incr_count; by move => ->. qed.
 
 lemma ec_incr_dom (cnts : 'a counts) (elem : 'a) :
-  dom(incr_count cnts elem) = dom cnts `|` fset1 elem.
+  fdom(incr_count cnts elem) = fdom cnts `|` fset1 elem.
 proof.
 rewrite /incr_count.
-case (mem (dom cnts) elem) => [mem_elem | not_mem_elem];
-by rewrite dom_set.
+case (elem \in cnts) => [elem_in_cnts | elem_not_in_cnts];
+by rewrite fdom_set.
 qed.
 
 lemma ec_get_not_in_dom (cnts : 'a counts) (elem : 'a) :
-  ! mem (dom cnts) elem => get_count cnts elem = 0.
-proof. smt(). qed.
+  ! elem \in cnts => get_count cnts elem = 0.
+proof. rewrite /get_count; by move => ->. qed.
 
 lemma ec_get_in_dom (cnts : 'a counts) (elem : 'a) :
-  mem (dom cnts) elem =>
-  get_count cnts elem = oget cnts.[elem].
-proof. smt(). qed.
+  elem \in cnts => get_count cnts elem = oget cnts.[elem].
+proof. rewrite /get_count; by move => ->. qed.
 
 lemma ec_get_empty (elem : 'a) :
   get_count empty_counts elem = 0.
-proof. by rewrite /get_count /empty_count dom0 in_fset0. qed.
+proof. by rewrite /get_count /empty_count mem_empty. qed.
 
 lemma ec_incr_oget_not_in_dom_eq (cnts : 'a counts) (elem : 'a) :
-  ! mem (dom cnts) elem =>
-  oget (incr_count cnts elem).[elem] = 1.
+  ! elem \in cnts => oget (incr_count cnts elem).[elem] = 1.
 proof.
-move => not_mem_dom_ec_elem; rewrite /incr_count.
-by rewrite not_mem_dom_ec_elem /= getP_eq oget_some.
+move => elem_not_in_cnts; rewrite /incr_count.
+by rewrite elem_not_in_cnts /= get_set_sameE oget_some.
 qed.
 
 lemma ec_incr_oget_in_dom_eq (cnts : 'a counts) (elem : 'a) :
-  mem (dom cnts) elem =>
+  elem \in cnts =>
   oget (incr_count cnts elem).[elem] = oget cnts.[elem] + 1.
 proof.
-move => mem_dom_ec_elem; rewrite /incr_count.
-case (mem (dom cnts) elem) => [mem_elem | not_mem_elem];
-  by rewrite getP /= oget_some.
+rewrite /incr_count; move => -> /=.
+by rewrite get_setE /= oget_some.
 qed.
 
 lemma ec_incr_get_eq (cnts : 'a counts) (elem : 'a) :
@@ -81,18 +78,20 @@ lemma ec_incr_get_eq (cnts : 'a counts) (elem : 'a) :
   get_count cnts elem + 1.
 proof.
 rewrite /get_count.
-case (mem (dom cnts) elem) => [mem | not_mem].
-by rewrite ec_incr_dom in_fsetU in_fset1 /= ec_incr_oget_in_dom_eq.
-by rewrite ec_incr_dom in_fsetU in_fset1 /= /incr_count not_mem /= getP.
+case (elem \in cnts) => [elem_in_cnts | elem_not_in_cnts].
+by rewrite -mem_fdom ec_incr_dom in_fsetU in_fset1 /= ec_incr_oget_in_dom_eq.
+by rewrite -mem_fdom ec_incr_dom in_fsetU in_fset1 /=
+           /incr_count elem_not_in_cnts /= get_set_sameE.
 qed.
 
 lemma ec_incr_oget_in_dom_ne (cnts : 'a counts) (elem elem' : 'a) :
-  elem' <> elem => mem (dom cnts) elem' =>
+  elem' <> elem => elem' \in cnts =>
   oget (incr_count cnts elem).[elem'] = oget cnts.[elem'].
 proof.
-move => ne_elem'_elem mem_dom_ec_elem'; rewrite /incr_count.
-case (mem (dom cnts) elem) => [mem_elem | not_mem_elem];
-  by rewrite getP ne_elem'_elem.
+move => ne_elem'_elem elem'_in_cnts; rewrite /incr_count.
+rewrite eq_sym in ne_elem'_elem.
+case (elem \in cnts) => [elem_in_cnts | elem_not_in_cnts];
+  by rewrite get_setE ne_elem'_elem //.
 qed.
 
 lemma ec_incr_get_ne (cnts : 'a counts) (elem elem' : 'a) :
@@ -101,9 +100,10 @@ lemma ec_incr_get_ne (cnts : 'a counts) (elem elem' : 'a) :
   get_count cnts elem'.
 proof.
 move => ne_elem'_elem; rewrite /get_count.
-rewrite ec_incr_dom in_fsetU in_fset1 ne_elem'_elem /=.
-case (mem (dom cnts) elem') => [mem_dom_ec_elem' | //];
-  by apply ec_incr_oget_in_dom_ne.
+rewrite -mem_fdom ec_incr_dom in_fsetU in_fset1 ne_elem'_elem /=
+         mem_fdom.
+case (elem' \in cnts) => [elem'_in_cnts | //].
+by apply ec_incr_oget_in_dom_ne.
 qed.
 
 lemma incr_count_swap (cnts : 'a counts, elem1 elem2 : 'a) :
@@ -111,53 +111,48 @@ lemma incr_count_swap (cnts : 'a counts, elem1 elem2 : 'a) :
   incr_count (incr_count cnts elem2) elem1.
 proof.
 case (elem1 = elem2) => [-> // | ne_elem1_elem2].
-case (mem (dom cnts) elem1) => [mem_ec_1 | not_mem_ec_1].
-case (mem (dom cnts) elem2) => [mem_ec_2 | not_mem_ec_2].
+case (elem1 \in cnts) => [elem1_in_cnts | elem1_not_in_cnts].
+case (elem2 \in cnts) => [elem2_in_cnts | elem2_not_in_cnts].
 do 2! rewrite (ec_incr_mem_eq cnts _) //.
-do 2! rewrite ec_incr_mem_eq 1:domP 1:in_fsetU1 1:/#.
-rewrite 2!getP ne_elem1_elem2; have -> /= : elem2 <> elem1 by smt().
-smt(set_set).
-rewrite (ec_incr_mem_eq cnts elem1) //.
-rewrite (ec_incr_not_mem_eq cnts elem2) //.
-rewrite (ec_incr_not_mem_eq _ elem2) 1:domP 1:in_fsetU1 1:/#.
-rewrite (ec_incr_mem_eq _ elem1) // 1:domP 1:in_fsetU1 1:/#.
-rewrite set_set ne_elem1_elem2 /=.
-by rewrite getP ne_elem1_elem2.
-case (mem (dom cnts) elem2) => [mem_ec_2 | not_mem_ec_2].
-rewrite (ec_incr_mem_eq cnts elem2) //.
-rewrite (ec_incr_not_mem_eq cnts elem1) //.
-rewrite (ec_incr_not_mem_eq _ elem1) 1:domP 1:in_fsetU1 1:/#.
-rewrite (ec_incr_mem_eq _ elem2) // 1:domP 1:in_fsetU1 1:/#.
-rewrite (set_set _ elem2 elem1); have -> // : elem2 <> elem1 by smt().
-rewrite getP; by have -> : elem2 <> elem1 by smt().
-do 2! rewrite (ec_incr_not_mem_eq cnts) //.
-do 2! rewrite ec_incr_not_mem_eq 1:domP 1:in_fsetU1 1:/#.
-smt(set_set).
+rewrite ec_incr_mem_eq 1:domE get_setE ne_elem1_elem2 //.
+by rewrite ec_incr_mem_eq 1:domE get_setE (eq_sym elem2 elem1)
+           ne_elem1_elem2 //= fmapSS_neqE.
+by rewrite (ec_incr_mem_eq cnts elem1) // (ec_incr_not_mem_eq cnts elem2) //
+           (ec_incr_not_mem_eq _ elem2) 1:domE 1:get_setE 1:ne_elem1_elem2 //
+           ec_incr_mem_eq 1:domE get_setE (eq_sym elem2 elem1)
+           ne_elem1_elem2 //= fmapSS_neqE.
+case (elem2 \in cnts) => [elem2_in_cnts | elem2_not_in_cnts].
+by rewrite (ec_incr_mem_eq cnts elem2) // (ec_incr_not_mem_eq cnts elem1) //
+           (ec_incr_not_mem_eq _ elem1) 1:domE 1:get_setE 1:(eq_sym elem2 elem1)
+           1:ne_elem1_elem2 // ec_incr_mem_eq 1:domE get_setE ne_elem1_elem2 //=
+           fmapSS_neqE.
+by rewrite (ec_incr_not_mem_eq cnts elem1) // (ec_incr_not_mem_eq cnts elem2) //
+           ec_incr_not_mem_eq 1:domE 1:get_setE 1:ne_elem1_elem2 //
+           ec_incr_not_mem_eq 1:domE 1:get_setE 1:(eq_sym elem2 elem1)
+           1:ne_elem1_elem2 // fmapSS_neqE 1:ne_elem1_elem2.
 qed.
 
 (* predicate preserved by incr_count *)
 
 pred dom_pos (cnts : 'a counts) =
   forall (elem : 'a),
-  mem (dom cnts) elem => 1 <= oget(cnts.[elem]).
+  elem \in cnts => 1 <= oget(cnts.[elem]).
 
 lemma dom_pos_empty : dom_pos empty_counts<:'a>.
-proof.
-move => elem.
-by rewrite dom0 in_fset0.
-qed.
+proof. move => elem; by rewrite mem_empty. qed.
 
 lemma dom_pos_incr (cnts : 'a counts, elem : 'a) :
   dom_pos cnts => dom_pos (incr_count cnts elem).
 proof.
-move => @/dom_pos dom_pos_ec elem' mem_incr_ec_elem_elem'.
-rewrite ec_incr_dom in_fsetU1 in mem_incr_ec_elem_elem'.
-elim mem_incr_ec_elem_elem' => [mem_ec_elem' | ->].
-have dom_pos_ec_elem' := dom_pos_ec elem' mem_ec_elem'.
+move => @/dom_pos dom_pos_ec elem' elem'_in_incr_cnts_elem.
+rewrite -mem_fdom ec_incr_dom in_fsetU mem_fdom
+        in_fset1 in elem'_in_incr_cnts_elem.
+elim elem'_in_incr_cnts_elem => [elem'_in_cnts | ->].
+have dom_pos_ec_elem' := dom_pos_ec elem' elem'_in_cnts.
 case (elem' = elem) => [<- | ne_elem'_elem].
 rewrite ec_incr_oget_in_dom_eq /#.
 by rewrite ec_incr_oget_in_dom_ne.
-case (mem (dom cnts) elem) => [mem_ec_elem | not_mem_ec_elem].
+case (elem \in cnts) => [elem_in_cnts | elem_not_in_cnts].
 rewrite ec_incr_oget_in_dom_eq /#.
 by rewrite ec_incr_oget_not_in_dom_eq.
 qed.
@@ -168,17 +163,23 @@ lemma counts_eq (cnts1 cnts2 : 'a counts) :
    get_count cnts1 elem = get_count cnts2 elem) =>
   cnts1 = cnts2.
 proof.
-move => dom_pos_ec1 dom_pos_ec2 get_count_eq.
-apply fmapP => elem.
-case (mem (dom cnts1) elem) => [mem_dom1_elem | not_mem_dom1_elem].
-case (mem (dom cnts2) elem) => [mem_dom2_elem | not_mem_dom2_elem].
+move => dom_pos_cnts1 dom_pos_cnts2 get_count_eq.
+apply fmap_eqP => elem.
+case (elem \in cnts1) => [elem_in_cnts1 | elem_not_in_cnts1].
+case (elem \in cnts2) => [elem_in_cnts2 | elem_not_in_cnts2].
 have get_count_eq_elem := get_count_eq elem.
-rewrite ec_get_in_dom // in get_count_eq_elem.
-rewrite ec_get_in_dom // in get_count_eq_elem.
-rewrite (get_oget cnts1) // (get_oget cnts2) //.
-smt().
-case (mem (dom cnts2) elem) => [mem_dom2_elem | not_mem_dom2_elem].
-smt().
+rewrite ec_get_in_dom // ec_get_in_dom // in get_count_eq_elem.
+rewrite (get_some cnts1 elem) // (get_some cnts2 elem) //.
 have get_count_eq_elem := get_count_eq elem.
-by rewrite get_none // get_none.
+rewrite (ec_get_in_dom cnts1 _ ) //
+        (ec_get_not_in_dom cnts2 _) // in get_count_eq_elem.
+have get_elem_cnts1_pos := dom_pos_cnts1 elem elem_in_cnts1.
+have // : 1 <= 0 by rewrite -get_count_eq_elem.
+case (elem \in cnts2) => [mem_dom2_elem | not_mem_dom2_elem].
+have get_count_eq_elem := get_count_eq elem.
+rewrite (ec_get_in_dom cnts2 _ ) //
+        (ec_get_not_in_dom cnts1 _) // in get_count_eq_elem.
+have get_elem_cnts2_pos := dom_pos_cnts2 elem mem_dom2_elem.
+have // : 1 <= 0 by rewrite get_count_eq_elem.
+do 2! rewrite get_none //.
 qed.
