MapAux.ec
@@ -1,0 +1,53 @@
+(* MapAux.ec *)
+
+require import AllCore SmtMap FSet.
+
+lemma get_none (mp : ('a, 'b) fmap, x : 'a) :
+  x \notin mp => mp.[x] = None.
+proof. by rewrite domE. qed.
+
+lemma get_some (mp : ('a, 'b) fmap, x : 'a) :
+  x \in mp => mp.[x] = Some (oget mp.[x]).
+proof. move => /domE; by case mp.[x]. qed.
+
+lemma set_same (mp : ('a, 'b) fmap, x : 'a) :
+  x \in mp => mp.[x <- oget mp.[x]] = mp.
+proof.
+move => x_in_mp.
+apply fmap_eqP => y.
+case (x = y) => [->> | ne_x_y].
+by rewrite get_set_sameE get_some.
+by rewrite get_setE ne_x_y.
+qed.
+
+lemma frng_set (mp : ('a, 'b) fmap, x : 'a, y : 'b) :
+  frng mp.[x <- y] = frng (rem mp x) `|` fset1 y.
+proof.
+apply fsetP => z; rewrite in_fsetU in_fset1 2!mem_frng 2!rngE /=.
+split => [[x'] | [[x'] | ->]].
+case (x = x') => [-> | ne_x_x'].
+by rewrite get_set_sameE /= => ->.
+rewrite get_setE ne_x_x' /= => get_x'_some_z.
+left; exists x'; by rewrite remE ne_x_x'.
+rewrite remE.
+case (x = x') => // ne_x_x' get_x'_some_z.
+exists x'; by rewrite get_setE ne_x_x'.
+exists x; by rewrite get_set_sameE.
+qed.
+
+lemma eq_except_ne_in (x y : 'a, mp1 mp2 : ('a, 'b) fmap) :
+  eq_except (pred1 x) mp1 mp2 => y <> x =>
+  y \in mp1 => y \in mp2.
+proof.
+move => /eq_exceptP @/pred1 eq_exc ne_y_x.
+by rewrite 2!domE eq_exc.
+qed.
+
+lemma rem_id (mp : ('a, 'b) fmap, x : 'a) :
+  x \notin mp => rem mp x = mp.
+proof.
+move => x_notin_mp; apply fmap_eqP => y; rewrite remE.
+case (x = y) => // <-.
+case (None = mp.[x]) => // get_not_none.
+rewrite eq_sym -domE // in get_not_none.
+qed.
